overhaul composition and Fin

ArkLib/OracleReduction/Composition/Sequential/Basic.lean
@@ -1,15 +1,14 @@
 /-
-Copyright (c) 2024 ArkLib Contributors. All rights reserved.
+Copyright (c) 2024-2025 ArkLib Contributors. All rights reserved.
 Released under Apache 2.0 license as described in the file LICENSE.
 Authors: Quang Dao
 -/
 
-import ArkLib.Data.Math.Fin
-import Batteries.Data.Fin.Fold
+import ArkLib.OracleReduction.Composition.Sequential.ProtocolSpec
 import ArkLib.OracleReduction.Security.Basic
 
 /-!
-  # Sequential Composition of (Oracle) Reductions
+  # Sequential Composition of Oracle Reductions
 
   We define the composition of two or more interactive (oracle) reductions, where the output
   statement & witness types for one reduction is the same as the input statement & witness types for
@@ -26,43 +25,6 @@ import ArkLib.OracleReduction.Security.Basic
 -/
 
 section find_home
-
-theorem cast_eq_cast_iff {α β γ : Sort _} {h : α = γ} {h' : β = γ} {a : α} {b : β} :
-    cast h a = cast h' b ↔ a = cast (h'.trans h.symm) b := by subst h'; subst h; simp
-
-theorem cast_symm {α β : Sort _} {h : α = β} {a : α} {b : β} :
-    cast h a = b ↔ a = cast h.symm b := by
-  subst h; simp
-
-theorem congrArg₃ {α β γ δ : Sort*} {f : α → β → γ → δ} {a a' : α} {b b' : β} {c c' : γ}
-    (h : a = a') (h' : b = b') (h'' : c = c') : f a b c = f a' b' c' := by
-  subst h; subst h'; subst h''; rfl
-
-theorem congrArg₄ {α β γ δ ε : Sort*} {f : α → β → γ → δ → ε} {a a' : α} {b b' : β} {c c' : γ}
-    {d d' : δ} (h : a = a') (h' : b = b') (h'' : c = c') (h''' : d = d') :
-      f a b c d = f a' b' c' d' := by
-  subst h; subst h'; subst h''; subst h'''; rfl
-
-namespace Fin
-
-variable {m n : ℕ} {α : Sort*}
-
-theorem append_left_injective (b : Fin n → α) : Function.Injective (@Fin.append m n α · b) := by
-  intro a a' h
-  simp only at h
-  ext i
-  have : append a b (castAdd n i) = append a' b (castAdd n i) := by rw [h]
-  simp only [append_left] at this
-  exact this
-
-theorem append_right_injective (a : Fin m → α) : Function.Injective (@Fin.append m n α a) := by
-  intro b b' h
-  ext i
-  have : append a b (natAdd m i) = append a b' (natAdd m i) := by rw [h]
-  simp only [append_right] at this
-  exact this
-
-end Fin
 
 variable {ι ι' : Type} {spec : OracleSpec ι} {spec' : OracleSpec ι'} {α β : Type}
     (oa : OracleComp spec α)
@@ -101,229 +63,6 @@ theorem tsum_cast {α β : Type u} {f : α → ENNReal} {g : β → ENNReal}
   subst h; simp [h']
 
 end find_home
-
-namespace ProtocolSpec
-
-/-! ### Restriction of Protocol Specifications & Transcripts -/
-
-section Restrict
-
-variable {n : ℕ}
-
-abbrev take (m : ℕ) (h : m ≤ n) (pSpec : ProtocolSpec n) := Fin.take m h pSpec
-
-abbrev rtake (m : ℕ) (h : m ≤ n) (pSpec : ProtocolSpec n) := Fin.rtake m h pSpec
-
-abbrev FullTranscript.take {pSpec : ProtocolSpec n} (m : ℕ) (h : m ≤ n)
-    (transcript : FullTranscript pSpec) : FullTranscript (pSpec.take m h) :=
-  Fin.take m h transcript
-
-abbrev FullTranscript.rtake {pSpec : ProtocolSpec n} (m : ℕ) (h : m ≤ n)
-    (transcript : FullTranscript pSpec) : FullTranscript (pSpec.rtake m h) :=
-  Fin.rtake m h transcript
-
-end Restrict
-
-section Cast
-
-def cast {n n' : ℕ} (h : n = n') (pSpec : ProtocolSpec n) : ProtocolSpec n' :=
-  pSpec ∘ (Fin.cast h.symm)
-
-@[simp]
-theorem cast_refl {n : ℕ} {h : n = n} : cast h = id := rfl
-
-@[simp]
-theorem cast_eq_self {n : ℕ} {pSpec : ProtocolSpec n} : cast (refl n) pSpec = pSpec := by
-  simp only [cast, Fin.cast_refl, CompTriple.comp_eq]
-
-@[simp]
-theorem cast_trans {n n' n'' : ℕ} {pSpec : ProtocolSpec n} (h : n = n') (h' : n' = n'') :
-    cast h' (cast h pSpec) = cast (h.trans h') pSpec := by
-  subst h; subst h'; simp only [cast, Fin.cast_refl, CompTriple.comp_eq]
-
-theorem cast_eq_cast_iff {n m k : ℕ} {pSpec : ProtocolSpec n} {pSpec' : ProtocolSpec m}
-    (h : n = k) (h' : m = k) :
-      cast h pSpec = cast h' pSpec' ↔ pSpec = cast (h'.trans h.symm) pSpec' := by
-  subst h; subst h'; simp only [cast, Fin.cast_refl, CompTriple.comp_eq]
-
-theorem cast_eq_root_cast {n m : ℕ} {pSpec : ProtocolSpec n} (h : n = m) :
-    cast h pSpec = _root_.cast (by simp [h]) pSpec := by subst h; simp only [cast_eq_self, cast_eq]
-
-end Cast
-
-/-! ### Composition of Two Protocol Specifications -/
-
-variable {m n : ℕ}
-
-/-- Adding a round with direction `dir` and type `Message` to the beginning of a `ProtocolSpec` -/
-abbrev cons (pSpec : ProtocolSpec n) (dir : Direction) (Message : Type) :
-    ProtocolSpec (n + 1) := Fin.cons ⟨dir, Message⟩ pSpec
-
-/-- Adding a round with direction `dir` and type `Message` to the end of a `ProtocolSpec` -/
-abbrev snoc (pSpec : ProtocolSpec n) (dir : Direction) (Message : Type) :
-    ProtocolSpec (n + 1) := Fin.snoc pSpec ⟨dir, Message⟩
-
-/-- Appending two `ProtocolSpec`s -/
-abbrev append (pSpec : ProtocolSpec m) (pSpec' : ProtocolSpec n) : ProtocolSpec (m + n) :=
-  Fin.append pSpec pSpec'
-
-@[inline, reducible]
-def mkSingle (dir : Direction) (Message : Type) : ProtocolSpec 1 := fun _ => ⟨dir, Message⟩
-
-infixl : 65 " ++ₚ " => ProtocolSpec.append
-
-@[simp]
-theorem append_cast_left {n m : ℕ} {pSpec : ProtocolSpec n} {pSpec' : ProtocolSpec m} (n' : ℕ)
-    (h : n = n') : (pSpec.cast h) ++ₚ pSpec' = (pSpec ++ₚ pSpec').cast (by omega) := by
-  simp only [append, cast, Fin.append_cast_left]
-
-/-- Reverse of non-prime version, to facilitate rewrite from the other side -/
-theorem append_cast_left' {n m : ℕ} {pSpec : ProtocolSpec n} {pSpec' : ProtocolSpec m} (n' : ℕ)
-    (h : n + m = n' + m) :
-      (pSpec ++ₚ pSpec').cast h = (pSpec.cast (Nat.add_right_cancel h)) ++ₚ pSpec' := by
-  simp only [append, cast, Fin.append_cast_left]
-
-@[simp]
-theorem append_cast_right {n m : ℕ} (pSpec : ProtocolSpec n) (pSpec' : ProtocolSpec m) (m' : ℕ)
-    (h : m = m') : pSpec ++ₚ (pSpec'.cast h) = (pSpec ++ₚ pSpec').cast (by omega) := by
-  simp only [append, cast, Fin.append_cast_right]
-
-/-- Reverse of non-prime version, to facilitate rewrite from the other side -/
-theorem append_cast_right' {n m : ℕ} (pSpec : ProtocolSpec n) (pSpec' : ProtocolSpec m) (m' : ℕ)
-    (h : n + m = n + m') :
-      (pSpec ++ₚ pSpec').cast h = pSpec ++ₚ (pSpec'.cast (Nat.add_left_cancel h)) := by
-  simp only [append, cast, Fin.append_cast_right]
-
-theorem append_left_injective {pSpec : ProtocolSpec n} :
-    Function.Injective (@ProtocolSpec.append m n · pSpec) :=
-  Fin.append_left_injective pSpec
-
-theorem append_right_injective {pSpec : ProtocolSpec m} :
-    Function.Injective (@ProtocolSpec.append m n pSpec) :=
-  Fin.append_right_injective pSpec
-
-@[simp]
-theorem append_left_cancel_iff {pSpec : ProtocolSpec n} {p1 p2 : ProtocolSpec m} :
-    p1 ++ₚ pSpec = p2 ++ₚ pSpec ↔ p1 = p2 :=
-  ⟨fun h => append_left_injective h, fun h => by rw [h]⟩
-
-@[simp]
-theorem append_right_cancel_iff {pSpec : ProtocolSpec m} {p1 p2 : ProtocolSpec n} :
-    pSpec ++ₚ p1 = pSpec ++ₚ p2 ↔ p1 = p2 :=
-  ⟨fun h => append_right_injective h, fun h => by rw [h]⟩
-
-@[simp]
-theorem snoc_take {pSpec : ProtocolSpec n} (k : ℕ) (h : k < n) :
-    (pSpec.take k (by omega) ++ₚ (fun (_ : Fin 1) => pSpec ⟨k, h⟩))
-      = pSpec.take (k + 1) (by omega) := by
-  simp only [append, take, Fin.append_right_eq_snoc, Fin.take_succ_eq_snoc]
-
-variable {pSpec₁ : ProtocolSpec m} {pSpec₂ : ProtocolSpec n}
-
-@[simp]
-theorem take_append_left :
-    (pSpec₁ ++ₚ pSpec₂).take m (Nat.le_add_right m n) = pSpec₁ := by
-  simp only [take, append]
-  have {i : Fin m} : Fin.castLE (by omega) i = Fin.castAdd n i := by
-    simp only [Fin.castLE, Fin.castAdd]
-  ext i <;>
-  simp only [Fin.take_apply, this, Fin.append_left]
-
-namespace FullTranscript
-
-/-- Appending two transcripts for two `ProtocolSpec`s -/
-def append (T₁ : FullTranscript pSpec₁) (T₂ : FullTranscript pSpec₂) :
-    FullTranscript (pSpec₁ ++ₚ pSpec₂) :=
-  fun i => (Fin.append_comp' Prod.snd i).mp (Fin.addCases' T₁ T₂ i)
-
-infixl : 65 " ++ₜ " => append
-
-/-- Adding a message with a given direction and type to the end of a `Transcript` -/
-def snoc {pSpec : ProtocolSpec n} {NextMessage : Type}
-    (T : FullTranscript pSpec) (dir : Direction) (msg : NextMessage) :
-        FullTranscript (pSpec ++ₚ .mkSingle dir NextMessage) :=
-  append T fun _ => msg
-
-theorem take_append_left (T : FullTranscript pSpec₁) (T' : FullTranscript pSpec₂) :
-    ((T ++ₜ T').take m (Nat.le_add_right m n)) =
-      (@take_append_left _ _ pSpec₁ pSpec₂).symm ▸ T := by
-  ext i
-  simp [take, append, ProtocolSpec.append]
-  simp [Fin.castLE, Fin.addCases', Fin.addCases]
-  -- refine heq_of_eq_cast ?_ ?_
-  sorry
-
-def fst (T : FullTranscript (pSpec₁ ++ₚ pSpec₂)) : FullTranscript pSpec₁ :=
-  fun i => by
-    simpa [ProtocolSpec.append, Fin.append_left] using T (Fin.castAdd n i)
-
-def snd (T : FullTranscript (pSpec₁ ++ₚ pSpec₂)) : FullTranscript pSpec₂ :=
-  fun i => by
-    simpa [ProtocolSpec.append, Fin.append_right] using T (Fin.natAdd m i)
-
-@[simp]
-theorem append_fst (T₁ : FullTranscript pSpec₁) (T₂ : FullTranscript pSpec₂) :
-    (T₁ ++ₜ T₂).fst = T₁ := by
-  funext i
-  simp [fst, append, eqRec_eq_cast]
-
-@[simp]
-theorem append_snd (T₁ : FullTranscript pSpec₁) (T₂ : FullTranscript pSpec₂) :
-    (T₁ ++ₜ T₂).snd = T₂ := by
-  funext i
-  simp [snd, append, eqRec_eq_cast]
-
-end FullTranscript
-
-def MessageIdx.inl (i : MessageIdx pSpec₁) : MessageIdx (pSpec₁ ++ₚ pSpec₂) :=
-  ⟨Fin.castAdd n i.1, by simpa only [Fin.append_left] using i.2⟩
-
-def MessageIdx.inr (i : MessageIdx pSpec₂) : MessageIdx (pSpec₁ ++ₚ pSpec₂) :=
-  ⟨Fin.natAdd m i.1, by simpa only [Fin.append_right] using i.2⟩
-
-@[simps!]
-def MessageIdx.sumEquiv :
-    MessageIdx pSpec₁ ⊕ MessageIdx pSpec₂ ≃ MessageIdx (pSpec₁ ++ₚ pSpec₂) where
-  toFun := Sum.elim (MessageIdx.inl) (MessageIdx.inr)
-  invFun := fun ⟨i, h⟩ => by
-    by_cases hi : i < m
-    · simp [ProtocolSpec.append, Fin.append, Fin.addCases, hi] at h
-      exact Sum.inl ⟨⟨i, hi⟩, h⟩
-    · simp [ProtocolSpec.append, Fin.append, Fin.addCases, hi] at h
-      exact Sum.inr ⟨⟨i - m, by omega⟩, h⟩
-  left_inv := fun i => by
-    rcases i with ⟨⟨i, isLt⟩, h⟩ | ⟨⟨i, isLt⟩, h⟩ <;>
-    simp [MessageIdx.inl, MessageIdx.inr, h, isLt]
-  right_inv := fun ⟨i, h⟩ => by
-    by_cases hi : i < m <;>
-    simp [MessageIdx.inl, MessageIdx.inr, hi]
-    congr; omega
-
-def ChallengeIdx.inl (i : ChallengeIdx pSpec₁) : ChallengeIdx (pSpec₁ ++ₚ pSpec₂) :=
-  ⟨Fin.castAdd n i.1, by simpa only [Fin.append_left] using i.2⟩
-
-def ChallengeIdx.inr (i : ChallengeIdx pSpec₂) : ChallengeIdx (pSpec₁ ++ₚ pSpec₂) :=
-  ⟨Fin.natAdd m i.1, by simpa only [Fin.append_right] using i.2⟩
-
-@[simps!]
-def ChallengeIdx.sumEquiv :
-    ChallengeIdx pSpec₁ ⊕ ChallengeIdx pSpec₂ ≃ ChallengeIdx (pSpec₁ ++ₚ pSpec₂) where
-  toFun := Sum.elim (ChallengeIdx.inl) (ChallengeIdx.inr)
-  invFun := fun ⟨i, h⟩ => by
-    by_cases hi : i < m
-    · simp [ProtocolSpec.append, Fin.append, Fin.addCases, hi] at h
-      exact Sum.inl ⟨⟨i, hi⟩, h⟩
-    · simp [ProtocolSpec.append, Fin.append, Fin.addCases, hi] at h
-      exact Sum.inr ⟨⟨i - m, by omega⟩, h⟩
-  left_inv := fun i => by
-    rcases i with ⟨⟨i, isLt⟩, h⟩ | ⟨⟨i, isLt⟩, h⟩ <;>
-    simp [ChallengeIdx.inl, ChallengeIdx.inr, h, isLt]
-  right_inv := fun ⟨i, h⟩ => by
-    by_cases hi : i < m <;>
-    simp [ChallengeIdx.inl, ChallengeIdx.inr, hi]
-    congr; omega
-
-end ProtocolSpec
 
 open ProtocolSpec
 
@@ -393,11 +132,6 @@ instance instSubSpecOfProtocolSpecAppendChallenge :
   --     simp only [PMF.map_apply, PMF.uniformOfFintype_apply, Fin.append_right]
   --     refine tsum_cast (by simp) (fun a => ?_)
   --     congr <;> try { simp only [Fin.append_right] } <;> symm <;> simp only [cast_heq]
-
--- instance {ι₁ ι₂ ι₃ : Type} {spec₁ : OracleSpec ι₁} {spec₂ : OracleSpec ι₂}
--- {spec₃ : OracleSpec ι₃}
---     [@SubSpec ι₁ ι₂ spec₁ spec₂] [@SubSpec ι₂ ι₃ spec₂ spec₃] :
--- @SubSpec ι₁ ι₃ spec₁ spec₃ := sorry
 
 instance : SubSpec [pSpec₁.Challenge]ₒ ([(pSpec₁ ++ₚ pSpec₂).Challenge]ₒ) where
   monadLift | query i t => instSubSpecOfProtocolSpecAppendChallenge.monadLift (query (Sum.inl i) t)
@@ -514,7 +248,8 @@ def Reduction.append (R₁ : Reduction pSpec₁ oSpec Stmt₁ Wit₁ Stmt₂ Wit
   prover := Prover.append R₁.prover R₂.prover
   verifier := Verifier.append R₁.verifier R₂.verifier
 
-variable [Oₘ₁ : ∀ i, OracleInterface (pSpec₁.Message i)] [Oₘ₂ : ∀ i, OracleInterface (pSpec₂.Message i)]
+variable [Oₘ₁ : ∀ i, OracleInterface (pSpec₁.Message i)]
+  [Oₘ₂ : ∀ i, OracleInterface (pSpec₂.Message i)]
   {ιₛ₁ : Type} {OStmt₁ : ιₛ₁ → Type} [Oₛ₁ : ∀ i, OracleInterface (OStmt₁ i)]
   {ιₛ₂ : Type} {OStmt₂ : ιₛ₂ → Type} [Oₛ₂ : ∀ i, OracleInterface (OStmt₂ i)]
   {ιₛ₃ : Type} {OStmt₃ : ιₛ₃ → Type} [Oₛ₃ : ∀ i, OracleInterface (OStmt₃ i)]
@@ -523,11 +258,23 @@ open Function Embedding in
 def OracleVerifier.append (V₁ : OracleVerifier pSpec₁ oSpec Stmt₁ Stmt₂ OStmt₁ OStmt₂)
     (V₂ : OracleVerifier pSpec₂ oSpec Stmt₂ Stmt₃ OStmt₂ OStmt₃) :
       OracleVerifier (pSpec₁ ++ₚ pSpec₂) oSpec Stmt₁ Stmt₃ OStmt₁ OStmt₃ where
-  verify := fun stmt challenges => sorry
+  verify := fun stmt challenges => by
+    -- First, invoke the first oracle verifier, handling queries as necessary
+    have := V₁.verify stmt (fun chal => sorry)
+    simp at this
+    -- Then, invoke the second oracle verifier, handling queries as necessary
+    -- Return the final output statement
+    sorry
 
-  embed := .trans V₂.embed <|
+  -- Need to provide an embedding `ιₛ₃ ↪ ιₛ₁ ⊕ (pSpec₁ ++ₚ pSpec₂).MessageIdx`
+  embed :=
+    -- `ιₛ₃ ↪ ιₛ₂ ⊕ pSpec₂.MessageIdx`
+    .trans V₂.embed <|
+    -- `ιₛ₂ ⊕ pSpec₂.MessageIdx ↪ (ιₛ₁ ⊕ pSpec₁.MessageIdx) ⊕ pSpec₂.MessageIdx`
     .trans (.sumMap V₁.embed (.refl _)) <|
+    -- re-associate the sum `_ ↪ ιₛ₁ ⊕ (pSpec₁.MessageIdx ⊕ pSpec₂.MessageIdx)`
     .trans (Equiv.sumAssoc _ _ _).toEmbedding <|
+    -- use the equivalence `pSpec₁.MessageIdx ⊕ pSpec₂.MessageIdx ≃ (pSpec₁ ++ₚ pSpec₂).MessageIdx`
     .sumMap (.refl _) MessageIdx.sumEquiv.toEmbedding
 
   hEq := fun i => by
@@ -536,6 +283,8 @@ def OracleVerifier.append (V₁ : OracleVerifier pSpec₁ oSpec Stmt₁ Stmt₂ 
       simp [h, h', V₁.hEq j, V₂.hEq i, MessageIdx.inl]
     · simp [h, V₂.hEq i, MessageIdx.inr]
 
+/-- Sequential composition of oracle reductions is just the sequential composition of the oracle
+  provers and oracle verifiers. -/
 def OracleReduction.append (R₁ : OracleReduction pSpec₁ oSpec Stmt₁ Wit₁ Stmt₂ Wit₂ OStmt₁ OStmt₂)
     (R₂ : OracleReduction pSpec₂ oSpec Stmt₂ Wit₂ Stmt₃ Wit₃ OStmt₂ OStmt₃) :
       OracleReduction (pSpec₁ ++ₚ pSpec₂) oSpec Stmt₁ Wit₁ Stmt₃ Wit₃ OStmt₁ OStmt₃ where
@@ -692,6 +441,13 @@ open OracleComp OracleSpec SubSpec
 variable [∀ i, Sampleable (pSpec₁.Challenge i)] [∀ i, Sampleable (pSpec₂.Challenge i)]
   [oSpec.DecidableEq]
 
+/--
+States that running an appended prover `P₁.append P₂` with an initial statement `stmt₁` and
+witness `wit₁` behaves as expected: it first runs `P₁` to obtain an intermediate statement
+`stmt₂`, witness `wit₂`, and transcript `transcript₁`. Then, it runs `P₂` on `stmt₂` and `wit₂`
+to produce the final statement `stmt₃`, witness `wit₃`, and transcript `transcript₂`.
+The overall output is `stmt₃`, `wit₃`, and the combined transcript `transcript₁ ++ₜ transcript₂`.
+-/
 theorem Prover.append_run (P₁ : Prover pSpec₁ oSpec Stmt₁ Wit₁ Stmt₂ Wit₂)
     (P₂ : Prover pSpec₂ oSpec Stmt₂ Wit₂ Stmt₃ Wit₃) (stmt : Stmt₁) (wit : Wit₁) :
       (P₁.append P₂).run stmt wit = (do
@@ -718,8 +474,12 @@ variable {pSpec₁ : ProtocolSpec m} {pSpec₂ : ProtocolSpec n} [∀ i, Samplea
     {rel₁ : Stmt₁ → Wit₁ → Prop} {rel₂ : Stmt₂ → Wit₂ → Prop} {rel₃ : Stmt₃ → Wit₃ → Prop}
     [oSpec.DecidableEq] [oSpec.FiniteRange]
 
-/-- If two reductions satisfy completeness with compatible relations, then their concatenation also
-  satisfies completeness with the sum of the completeness errors. -/
+/-- If two reductions satisfy completeness with compatible relations (`rel₁`, `rel₂` for `R₁` and
+    `rel₂`, `rel₃` for `R₂`), and respective completeness errors `completenessError₁` and
+    `completenessError₂`, then their sequential composition `R₁.append R₂` also satisfies
+    completeness with respect to `rel₁` and `rel₃`.
+    The completeness error of the appended reduction is the sum of the individual errors
+    (`completenessError₁ + completenessError₂`). -/
 theorem completeness_append (R₁ : Reduction pSpec₁ oSpec Stmt₁ Wit₁ Stmt₂ Wit₂)
     (R₂ : Reduction pSpec₂ oSpec Stmt₂ Wit₂ Stmt₃ Wit₃)
     {completenessError₁ completenessError₂ : ℝ≥0}
